[ffi] Flatten command line arguments.
Command line arguments to any program following the C calling convention
comprises of 2 parts:
* the number of arguments(including the program name).
* the arguments themselves(as a vector - an array of character arrays)

This patch stores these values in a global address and then flattens the
vector to a byte array, where each argument is separated by a '\0' and
the byte array ends with a series of 3 '\0' characters.

For example, the vector:
argv[][] = {
  "progname",
  "arg1",
  "arg2",
  "arg3"
};

Will be flattened to look like:

char * args = "progname\0arg1\0arg2\0arg3\0\0\0";

The flattening of the vector is done in C.

The assembly side of things is only done for x86_64 for now, Need to implement
arm6, arm8, riscv and mips support.

compiler/bootstrap/io/io_ffi.c
@@ -1,4 +1,12 @@
 #include <stdio.h>
+#include <string.h>
+
+/*
+  argc and argv are exported from cake.S
+ */
+extern int argc;
+extern char **argv;
+
 
 void ffiputChar (char* a) {
   putchar(a[0]);
@@ -12,4 +20,19 @@ void ffigetChar (char* a) {
     a[0] = c;
     a[1] = 0;
   }
+}
+
+/* NOTE: 256 corresponds to the length of 'a' in the basis library */
+#define MAXLEN 256
+
+void ffigetArgs (char *a) {
+        int i, j, k;
+
+        for (i = 0, k = 0; (i < argc) && (k < MAXLEN); i++, k++) {
+                for (j = 0; j < strlen(argv[i]) && (k+1 < MAXLEN); j++) {
+                        a[k++] = argv[i][j];
+                }
+        }
+
+        return;
 }
